pk_dh.v
@@ -1,0 +1,98 @@
+From stdpp Require Import base gmap.
+From mathcomp Require Import ssreflect.
+From iris.algebra Require Import agree auth csum gset gmap excl frac.
+From iris.heap_lang Require Import notation proofmode.
+From cryptis Require Import lib term cryptis primitives tactics role nown dh.
+From cryptis Require Import pk_auth.
+From cryptis Require Import session.
+
+Set Implicit Arguments.
+Unset Strict Implicit.
+Unset Printing Implicit Defensive.
+
+Section PKDH.
+
+Context `{heap : !heapGS Σ, cryptis : !cryptisG Σ, sess : !sessionG Σ}.
+Notation iProp := (iProp Σ).
+Implicit Types rl : role.
+Implicit Types t kI kR nI nR sI sR : term.
+
+Definition pk_dh_mk_key_share n := TExp (TInt 0) [n].
+
+Definition pk_dh_mk_key_share_impl : val := λ: <>,
+  let: "n" := mknonce #() in
+  ("n", texp (tgroup (tint #0)) "n").
+
+Definition pk_dh_mk_session_key rl n s : term :=
+  Spec.texp s n.
+
+Definition pk_dh_mk_session_key_impl rl : val :=
+  λ: "n" "s", texp "s" "n".
+
+Variable N : namespace.
+
+Program Instance PK_DH : PK := {
+  is_priv_key n kI kR := (
+    □ (pterm n ↔ ▷ False) ∧
+    □ (∀ s, dh_pred n s ↔ ▷ corruption kI kR)
+  )%I;
+
+  mk_key_share := pk_dh_mk_key_share;
+  mk_key_share_impl := pk_dh_mk_key_share_impl;
+  mk_session_key := pk_dh_mk_session_key;
+  mk_session_key_impl := pk_dh_mk_session_key_impl;
+
+}.
+
+Next Obligation.
+by move=> t1 t2 /TExp_inj [_ /(Permutation_singleton_inj _ _) t1t2].
+Qed.
+
+Next Obligation.
+move=> n; rewrite sterm_TExp /= sterm_TInt. apply: anti_symm.
+- by iIntros "(_ & ? & _)".
+- by eauto.
+Qed.
+
+Next Obligation.
+iIntros "%nI %kI %kR #s_nI [#p_nI #dh]".
+rewrite /pk_dh_mk_key_share /secret_of pterm_TExp1 sterm_TInt.
+iModIntro. iSplit.
+- iIntros "(_ & _ & #[contra|p_sI])".
+  + iDestruct ("p_nI" with "contra") as ">[]".
+  + iApply "dh". by eauto.
+- iIntros "#fail". do !iSplit => //. iRight. by iApply "dh".
+Qed.
+
+Next Obligation.
+move=> nI nR; rewrite /pk_dh_mk_key_share /pk_dh_mk_session_key.
+by rewrite !Spec.texpA TExpC2.
+Qed.
+
+Next Obligation.
+iIntros "%rl %t1 %t2 #s_t1 #s_t2".
+by rewrite /pk_dh_mk_session_key; iApply sterm_texp.
+Qed.
+
+Next Obligation.
+iIntros "%E %kI %kR %Φ _ post". rewrite /pk_dh_mk_key_share_impl.
+wp_pures. wp_bind (mknonce _).
+iApply (wp_mknonce _ (λ _, False)%I (λ _, corruption kI kR)).
+iIntros "%n #s_n #p_n #dh token". wp_pures.
+wp_bind (tint _). iApply wp_tint.
+wp_bind (tgroup _). iApply wp_tgroup.
+wp_bind (texp _ _). iApply wp_texp. rewrite Spec.texpA.
+wp_pures. iModIntro. iApply "post".
+rewrite bi.intuitionistic_intuitionistically.
+iFrame. iSplit => //. iSplit => //. iModIntro.
+iIntros "%t". iSpecialize ("dh" $! t).
+by rewrite bi.intuitionistic_intuitionistically.
+Qed.
+
+Next Obligation.
+iIntros "%E %rl %n %s %Φ _ post".
+rewrite /pk_dh_mk_session_key_impl.
+wp_pures. iApply wp_texp. by iApply "post".
+Qed.
+
+End PKDH.
